finish fsub/autosubst2_sctx subtyping_transitivity and subtyping_subst

fsub/autosubst2_sctx/prop_basic.v
@@ -75,3 +75,84 @@ Proof.
   - eapply ctx_tvar_rename_weak_rebounding; eauto.
   - asimpl; auto.
 Qed.
+
+Lemma sub_renaming_tvar Δ Δ' A B ξ :
+  Δ ⊢ A <: B ->
+  ctx_tvar_rename Δ Δ' ξ ->
+  Δ' ⊢ A ⟨ ξ ⟩ <: B ⟨ ξ ⟩.
+Proof.
+  move => H.
+  move: Δ' ξ. elim: Δ A B / H; intros; 
+    try hauto unfold:ctx_tvar_rename,ctx_tvar_rename_weak ctrs:subtyping use:wf_typ_renaming_tvar.
+  - asimpl. eapply sub_all; try hauto unfold:ctx_tvar_rename,ctx_tvar_rename_weak ctrs:subtyping use:wf_typ_renaming_tvar.
+    eapply H0.
+    unfold ctx_tvar_rename in *. intros. asimpl. simpl in *.
+    inversion H2; subst; asimpl.
+    + replace (ren_typ (ξ >> S) B1) with (B1 ⟨ξ⟩ ⟨S⟩) by (asimpl; auto).
+      constructor.
+    + replace (ren_typ (ξ >> S) A) with (A ⟨ξ⟩ ⟨S⟩) by (asimpl; auto).
+      constructor; eauto.
+Qed.
+
+Corollary sub_weakening_tvar0 Δ A B C:
+  Δ ⊢ A <: B ->
+  (entry_tvar C :: Δ) ⊢ A ⟨↑⟩ <: B ⟨↑⟩.
+Proof.
+  hauto unfold:ctx_tvar_rename ctrs:subtyping use:sub_renaming_tvar ctrs:lookup_tvar.
+Qed.
+
+Lemma sub_wf_typ Δ A B :
+  Δ ⊢ A <: B ->
+  (Δ ⊢ A) /\ (Δ ⊢ B).
+Proof.
+  intros; induction H; try hauto.
+  - simpl; repeat split; try hauto.
+    replace (A2) with (A2 ⟨id⟩) by (asimpl; auto).
+    hauto unfold:ctx_tvar_rename_weak 
+      inv:lookup_tvar ctrs:lookup_tvar use:wf_typ_renaming_tvar.
+Qed.
+
+Corollary sub_wf_typ1 Δ A B :
+  Δ ⊢ A <: B ->
+  Δ ⊢ A.
+Proof.
+  hauto use:sub_wf_typ.
+Qed.
+
+Corollary sub_wf_typ2 Δ A B :
+  Δ ⊢ A <: B ->
+  Δ ⊢ B.
+Proof.
+  hauto use:sub_wf_typ.
+Qed.
+
+Definition ctx_var_rename Γ Γ' ξ ζ :=
+  forall x A, lookup_var x Γ A -> lookup_var (ζ x) Γ' (A ⟨ ξ ⟩).
+
+(* Fixpoint map_entry_tvar (f: typ -> typ) (Γ: list entry) :=
+  match Γ with
+  | nil => nil
+  | (entry_tvar A) :: Γ' => (entry_tvar (f A)) :: (map_entry_tvar f Γ')
+  | (entry_var A) :: Γ' => (entry_var A) :: (map_entry_tvar f Γ')
+  end.
+
+Fixpoint map_entry_var (f: typ -> typ) (Γ: list entry) :=
+  match Γ with
+  | nil => nil
+  | (entry_tvar A) :: Γ' => (entry_tvar A) :: (map_entry_var f Γ')
+  | (entry_var A) :: Γ' => (entry_var (f A)) :: (map_entry_var f Γ')
+  end.
+
+Lemma lookup_map : forall A f Γ x ,
+  lookup_var x Γ A -> lookup_var x (map_entry_var f Γ) (f A).
+Proof.
+  intros.  generalize dependent f. induction H; simpl; auto using lookup_var.
+  - intros. eapply skip_tvar. econstructor.
+Qed.
+
+Lemma lookup_var_map_inv : forall x A' f Γ,
+  lookup_var x (map f Γ) A' -> exists A, A' = (f A) /\ lookup_var x Γ A.
+Proof.
+  intros. dependent induction H; 
+    destruct Γ; hauto inv:lookup_var ctrs:lookup_var.
+Qed. *)
