fsub/autosubst2_sctx/prop_subtyping.v
@@ -1,0 +1,190 @@
+Require Import common.prop_as_core.
+Require Import common.prop_as_unscoped.
+Require Import fsub.autosubst2_sctx.def_as2.
+Require Import fsub.autosubst2_sctx.def_extra.
+Require Import fsub.autosubst2_sctx.prop_basic.
+
+From Coq Require Import ssreflect ssrfun ssrbool.
+From Hammer Require Import Tactics.
+Require Import Coq.Program.Equality.
+Require Import List.
+Require Import Arith.
+
+Import SubstNotations.
+Import UnscopedNotations.
+
+Fixpoint typ_size (A : typ) :=
+  match A with
+  | typ_arr A B => 1 + typ_size A + typ_size B
+  | typ_all A B => 1 + typ_size A + typ_size B
+  | _ => 0
+  end.
+
+Lemma typ_size_renaming_eq A ξ:
+  typ_size (A ⟨ ξ ⟩) = typ_size A.
+Proof.
+  move : ξ; induction A; intros; simpl; hauto.
+Qed.
+
+Lemma lookup_tvar_det : forall Δ X A B,
+  lookup_tvar X Δ A -> lookup_tvar X Δ B -> A = B.
+Proof.
+  intros. move : B H0. 
+    induction H; hauto inv:lookup_tvar ctrs:lookup_tvar.
+Qed.
+
+Fixpoint num_tvars (Δ : ctx) :=
+  match Δ with
+  | nil => 0
+  | entry_tvar _ :: Δ => 1 + num_tvars Δ
+  | _ :: Δ => num_tvars Δ
+  end.
+
+Corollary ctx_tvar_renaming_tvars Δ1 Δ2 A: 
+  ctx_tvar_rename Δ1 (Δ2 ++ (entry_tvar A) :: Δ1) (fun X : nat => 1 + (num_tvars Δ2 + X)).
+Proof.
+  intros. unfold ctx_tvar_rename. intros.
+    induction Δ2; simpl; try hauto inv:lookup_tvar ctrs:lookup_tvar.
+  - destruct a; eauto using lookup_tvar.
+    replace (⟨fun X0 : nat => S (S (num_tvars Δ2 + X0))⟩ B) with
+    (B ⟨fun X : nat => 1 + (num_tvars Δ2 + X)⟩ ⟨ ↑⟩ ) by (asimpl; eauto).
+    eauto using lookup_tvar.
+Qed.
+
+Lemma lookup_tvar_rebounding : forall Δ1 Δ2 B,
+  lookup_tvar (num_tvars Δ2) (Δ2 ++ (entry_tvar B) :: Δ1) (B ⟨fun X => 1 + (num_tvars Δ2 + X) ⟩) /\
+  (forall X A B', X <> num_tvars Δ2 -> 
+    lookup_tvar X (Δ2 ++ (entry_tvar B) :: Δ1) A ->
+    lookup_tvar X (Δ2 ++ (entry_tvar B') :: Δ1) A).
+Proof.
+  split. 
+  - induction Δ2; simpl; asimpl; try hauto ctrs:lookup_tvar.
+    + destruct a; try hauto ctrs:lookup_tvar. 
+      replace (ren_typ (Init.Nat.add (S (num_tvars Δ2)) >> S) B) with
+      (B ⟨fun X : nat => 1 + (num_tvars Δ2 + X)⟩ ⟨↑⟩ ) by (asimpl; auto).
+      hauto ctrs:lookup_tvar. 
+  - intros. dependent induction H0.
+    + destruct Δ2; simpl in *; try hauto ctrs:lookup_tvar.
+    + destruct Δ2; simpl in *; try hauto ctrs:lookup_tvar.
+    + destruct Δ2; simpl in *; try hauto ctrs:lookup_tvar.
+Qed.
+
+Lemma conj' (A B : Prop) : A -> (A -> B) -> A /\ B.
+Proof. tauto. Qed.
+
+Theorem subtyping_reflexivity Δ A :
+  Δ ⊢ A ->
+  Δ ⊢ A <: A.
+Proof.
+  move : Δ. induction A; intros; try hauto ctrs:subtyping.
+  - apply sub_top; auto.
+Qed.
+
+(* the size function is to relate B and (B ⟨ξ⟩) (more concretely, B and (B ⟨↑ >> ↑ ... >> ↑⟩) )
+   (this is a debrujin specific issue, I believe)
+   a more direct generalization to achieve this can be found at
+   https://www.ps.uni-saarland.de/extras/autosubst2/poplmark/html/POPLMark.POPLMark.html#sub_trans'
+   (this may only work in the well-scoped version)
+*)
+Theorem subtyping_transitivity_narrowing n:
+  (forall Δ A B C,  
+    typ_size B = n -> 
+    Δ ⊢ A <: B ->
+    Δ ⊢ B <: C ->
+    Δ ⊢ A <: C) /\
+  (forall Δ1 Δ2 A B B' C,
+    typ_size B = n -> 
+    Δ2 ++ (entry_tvar B :: Δ1) ⊢ A <: C ->
+    Δ1 ⊢ B' <: B ->
+    Δ2 ++ (entry_tvar B' :: Δ1) ⊢ A <: C).
+Proof.
+  induction (lt_wf n) as [n _ IH].
+  intros. apply conj'.
+  - intros. move : C H1. induction H0; intros; try hauto ctrs:subtyping.
+    + inversion H1; subst.
+      * hauto ctrs:subtyping. 
+    + simpl in *. 
+      inversion H1; subst.
+      * eapply sub_top. hauto use:sub_wf_typ1, sub_wf_typ2.
+      * eapply sub_arrow.
+        -- edestruct (IH (typ_size B1)). hfcrush. hauto. 
+        -- edestruct (IH (typ_size B2)). hfcrush. hauto. 
+    + inversion H1; subst.
+      * eapply sub_top. simpl in *. split.
+        -- hauto use:sub_wf_typ1, sub_wf_typ2.
+        -- eapply wf_typ_renaming_tvar' with (ξ:=id) (A:=A2) (A':=A2) (Δ:=(entry_tvar B1)::Δ);
+          hauto unfold:ctx_tvar_rename_weak inv:lookup_tvar ctrs:lookup_tvar use:sub_wf_typ1, sub_wf_typ2 simp+:asimpl.
+      * eapply sub_all; eauto.
+        -- edestruct (IH (typ_size B1)). hfcrush. auto. hauto. 
+        -- edestruct (IH (typ_size B1)). eauto. hfcrush. eauto. 
+           edestruct (IH (typ_size B2)). hfcrush. eauto.
+           replace ((entry_tvar B0) :: Δ) with (nil ++ (entry_tvar B0) :: Δ) by auto.
+           eapply H2; eauto.
+  - intros Htrans. intros. move : B' H1. dependent induction H0; intros; auto.
+    + eapply sub_top.
+      eapply wf_typ_renaming_tvar' with (ξ:=id); 
+        hauto use:ctx_tvar_rename_weak_rebounding simp+:asimpl.
+    + eapply sub_tvar_refl; eauto.
+      eapply wf_typ_renaming_tvar' with (ξ:=id) (A:=typ_var X); 
+        hauto use:ctx_tvar_rename_weak_rebounding simp+:asimpl.
+    + edestruct (Nat.eq_dec X (num_tvars Δ2)).
+      * subst. 
+        eapply sub_tvar_bound with (A:=B' ⟨fun X => 1 + (num_tvars Δ2 + X) ⟩).
+        hauto use:lookup_tvar_rebounding. eapply Htrans with (B:=B ⟨fun X => 1 + (num_tvars Δ2 + X) ⟩).
+        -- hauto use:typ_size_renaming_eq.
+        -- eapply sub_renaming_tvar; eauto.
+           eapply ctx_tvar_renaming_tvars.
+        -- erewrite (lookup_tvar_det _ _ (⟨fun X : nat => 1 + (num_tvars Δ2 + X)⟩ B)); eauto.
+           hauto use:lookup_tvar_rebounding.
+      * subst. eapply sub_tvar_bound; eauto.
+        eapply lookup_tvar_rebounding; eauto.
+    + hauto ctrs:subtyping.
+    + eapply sub_all; try hauto ctrs:subtyping.
+      * eapply wf_typ_renaming_tvar' with (ξ:=id); 
+        hauto use:ctx_tvar_rename_weak_rebounding simp+:asimpl.
+      * replace ((entry_tvar B1) :: Δ2 ++ (entry_tvar B') :: Δ1) with ((entry_tvar B1 :: Δ2) ++ (entry_tvar B') :: Δ1) by auto.
+        eapply IHsubtyping2; eauto.
+Qed.
+
+Corollary subtyping_transitivity Δ A B C:
+  Δ ⊢ A <: B -> 
+  Δ ⊢ B <: C -> 
+  Δ ⊢ A <: C.
+Proof.
+  eapply subtyping_transitivity_narrowing; eauto.
+Qed.
+
+Corollary subtyping_narrowing Δ1 Δ2 A B B' C:
+  Δ2 ++ (entry_tvar B) :: Δ1 ⊢ A <: C ->
+  Δ1 ⊢ B' <: B ->
+  Δ2 ++ (entry_tvar B') :: Δ1 ⊢ A <: C.
+Proof.
+  eapply subtyping_transitivity_narrowing; eauto.
+Qed.
+
+Definition ctx_tvar_subst Δ Δ' σ :=
+  forall X A, lookup_tvar X Δ A -> Δ' ⊢ σ X <: A [σ].
+
+Lemma subtyping_subst Δ Δ' A B σ :
+  Δ ⊢ A <: B ->
+  ctx_tvar_subst Δ Δ' σ ->
+  Δ' ⊢ A [ σ ] <: B [ σ ].
+Proof.
+  move => H. move : Δ' σ. elim: Δ A B / H; intros.
+  - asimpl.
+    hauto unfold:ctx_tvar_subst_wf,ctx_tvar_subst use:wf_typ_subst_tvar,sub_wf_typ1,sub_wf_typ2 ctrs:subtyping.
+  - hauto use:subtyping_reflexivity,sub_wf_typ1 unfold:ctx_tvar_subst ctrs:subtyping.
+  - hauto use:subtyping_transitivity unfold:ctx_tvar_subst ctrs:subtyping.
+  - apply sub_arrow; hauto.
+  - asimpl. apply sub_all; eauto.
+    + hauto unfold:ctx_tvar_subst_wf,ctx_tvar_subst use:wf_typ_subst_tvar,sub_wf_typ1,sub_wf_typ2 ctrs:subtyping.
+    + apply H0. unfold ctx_tvar_subst in *. intros.
+      inversion H2; subst; asimpl.
+      eapply sub_tvar_bound with (A:=B1 [σ] ⟨ ↑ ⟩). econstructor.
+      replace (subst_typ (σ >> (ren_typ ↑)) B1) with (B1 [σ] ⟨ ↑ ⟩) by (asimpl; auto).
+      eapply sub_weakening_tvar0. 
+      hauto unfold:ctx_tvar_subst_wf inv:lookup_tvar ctrs:lookup_tvar use:sub_wf_typ1,sub_wf_typ2,subtyping_reflexivity,wf_typ_subst_tvar.
+      replace (subst_typ (σ >> (ren_typ ↑)) A0) with (A0 [σ] ⟨ ↑ ⟩) by (asimpl; auto).
+      eapply sub_weakening_tvar0. 
+      hauto unfold:ctx_tvar_subst_wf inv:lookup_tvar ctrs:lookup_tvar use:sub_wf_typ1,sub_wf_typ2,subtyping_reflexivity,wf_typ_subst_tvar.
+Qed.
